sepcomp-reserved/extension_proof.v
@@ -148,41 +148,34 @@ split3; auto.
 solve[exists n; eauto].
 Qed.
 
-Lemma private_block_dec: forall i x b,
-  {private_block (csem i) x b}+{~private_block (csem i) x b}.
-Proof.
-intros.
-apply private_dec; auto.
-Qed.
-
-Lemma private_valid_inv:
+Lemma owned_valid_inv:
   forall s s' (x x': cT (active E s)) m m' n,
   proj_core E (active E s) s = Some x -> 
-  private_valid esem csem E s m -> 
+  owned_valid esem csem E s m -> 
   corestepN (csem (active E s)) (genv_map (active E s)) n x m x' m' -> 
   corestepN esem ge n s m s' m' -> 
   proj_core E (active E s) s' = Some x' ->
-  private_valid esem csem E s' m'.
+  owned_valid esem csem E s' m'.
 Proof.
 intros until n; intros H1 H2 H3 H4 H5.
-intros i x'' PROJ b PRIV.
+intros i x'' PROJ b ofs PRIV.
 assert (H6: Mem.nextblock m <= Mem.nextblock m').
  apply corestepN_fwd in H3.
  solve[apply forward_nextblock in H3; auto].
 destruct (eq_nat_dec i (active E s)). subst.
 rewrite PROJ in H5; inv H5.
-assert (H5: {private_block (csem (active E s)) x b}+
-            {~private_block (csem (active E s)) x b}) 
- by apply private_block_dec.
+assert (H5: {owned (csem (active E s)) x b ofs}+
+            {~owned (csem (active E s)) x b ofs}) 
+ by apply owned_dec.
 destruct H5 as [H5|H5].
-specialize (H2 (active E s) x H1 b H5).
+specialize (H2 (active E s) x H1 b ofs H5).
 omega.
-eapply private_newN in PRIV; eauto.
+eapply owned_newN in PRIV; eauto.
 solve[destruct PRIV; auto].
 
 cut (proj_core E i s = Some x''). intro H7.
-unfold private_valid in H2.
-specialize (H2 i x'' H7 b PRIV).
+unfold owned_valid in H2.
+specialize (H2 i x'' H7 b ofs PRIV).
 assert (H8: Mem.nextblock m <= Mem.nextblock m').
  apply corestepN_fwd in H3.
  solve[apply forward_nextblock in H3; auto].
@@ -191,35 +184,42 @@ inv Hcore_compatible.
 solve[erewrite corestep_others_backward; eauto].
 Qed.
 
-Lemma private_valid_after_ext: 
+Lemma owned_dec: forall i x b ofs,
+  {owned (csem i) x b ofs}+{~owned (csem i) x b ofs}.
+Proof.
+intros.
+apply owned_dec; auto.
+Qed.
+
+Lemma owned_valid_after_ext: 
   forall s s' (x x': cT (active E s)) m m' ef sig args retv, 
   proj_core E (active E s) s = Some x -> 
-  private_valid esem csem E s m -> 
+  owned_valid esem csem E s m -> 
   at_external (csem (active E s)) x = Some (ef, sig, args) -> 
   after_external (csem (active E s)) retv x = Some x' -> 
   after_external esem retv s = Some s' -> 
   proj_core E (active E s) s' = Some x' ->
   mem_forward m m' -> 
-  private_valid esem csem E s' m'.
+  owned_valid esem csem E s' m'.
 Proof.
 intros until retv; intros PROJ PRIV AT AFTER AFTER' PROJ' FWD.
-intros i c PROJC b PRIVB.
+intros i c PROJC b ofs PRIVB.
 destruct (eq_nat_dec i (active E s)).
 subst.
-destruct (private_block_dec x b). 
-unfold private_valid in PRIV.
+destruct (owned_dec x b ofs). 
+unfold owned_valid in PRIV.
 cut (b < Mem.nextblock m). intro H1.
 cut (Mem.nextblock m <= Mem.nextblock m'). intro H2.
 omega.
 solve[apply forward_nextblock in FWD; auto].
 eapply PRIV; eauto.
 rewrite PROJC in PROJ'; inv PROJ'.
-eapply private_external in AFTER; eauto.
+eapply owned_external in AFTER; eauto.
 solve[elimtype False; eauto].
 assert (proj_core E i s = Some c).
  inv Hcore_compatible.
  rewrite after_ext_others with (retv := retv) (s' := s'); auto.
-unfold private_valid in PRIV.
+unfold owned_valid in PRIV.
 cut (b < Mem.nextblock m). intro H1.
 cut (Mem.nextblock m <= Mem.nextblock m'). intro H2.
 omega.
@@ -227,24 +227,24 @@ solve[apply forward_nextblock in FWD; auto].
 solve[eapply PRIV; eauto].
 Qed.
 
-Lemma private_disjoint_after_ext: 
+Lemma owned_disjoint_after_ext: 
   forall s s' (x x': cT (active E s)) ef sig args retv, 
   proj_core E (active E s) s = Some x -> 
-  private_disjoint esem csem E s -> 
+  owned_disjoint esem csem E s -> 
   at_external (csem (active E s)) x = Some (ef, sig, args) -> 
   after_external (csem (active E s)) retv x = Some x' -> 
   after_external esem retv s = Some s' -> 
   proj_core E (active E s) s' = Some x' ->
-  private_disjoint esem csem E s'.
+  owned_disjoint esem csem E s'.
 Proof.
 intros until retv; intros PROJ PRIV AT AFTER AFTER' PROJ'.
-unfold private_disjoint.
-intros until d; intros NEQ PROJC PROJD b PRIVATE CONTRA.
+unfold owned_disjoint.
+intros until d; intros NEQ PROJC PROJD b ofs PRIVATE CONTRA.
 destruct (eq_nat_dec i (active E s)).
 subst.
 rewrite PROJ' in PROJC.
 inv PROJC.
-eapply private_external in PRIVATE; eauto.
+eapply owned_external in PRIVATE; eauto.
 inv Hcore_compatible.
 eapply after_ext_others in AFTER'; eauto.
 rewrite <-AFTER' in *; clear AFTER'.
@@ -253,7 +253,7 @@ destruct (eq_nat_dec j (active E s)).
 subst.
 rewrite PROJ' in PROJD.
 inv PROJD.
-eapply private_external in CONTRA; eauto.
+eapply owned_external in CONTRA; eauto.
 inv Hcore_compatible.
 apply after_ext_others with (j := i) in AFTER'; eauto.
 rewrite <-AFTER' in *; clear AFTER'.
@@ -264,45 +264,45 @@ apply after_ext_others with (j := i) in AFTER'; eauto.
 apply after_ext_others with (j := j) in AFTER''; eauto.
 rewrite <-AFTER' in *; clear AFTER'.
 rewrite <-AFTER'' in *; clear AFTER''.
-specialize (PRIV i j c d NEQ PROJC PROJD b PRIVATE CONTRA).
+specialize (PRIV i j c d NEQ PROJC PROJD b ofs PRIVATE CONTRA).
 solve[auto].
 Qed.
 
-Lemma private_disjoint_inv:
+Lemma owned_disjoint_inv:
   forall s s' (x x': cT (active E s)) m m' n,
   proj_core E (active E s) s = Some x -> 
-  private_valid esem csem E s m -> 
-  private_disjoint esem csem E s -> 
+  owned_valid esem csem E s m -> 
+  owned_disjoint esem csem E s -> 
   corestepN (csem (active E s)) (genv_map (active E s)) n x m x' m' -> 
   corestepN esem ge n s m s' m' -> 
   proj_core E (active E s) s' = Some x' ->
-  private_disjoint esem csem E s'.
+  owned_disjoint esem csem E s'.
 Proof. 
 intros until n; intros H1 VAL H2 H3 H4 H5.
 intros i j c d H6 H7 H8.
 destruct (eq_nat_dec i (active E s)). subst.
 cut (proj_core E j s = Some d). intro H9.
 rewrite H5 in H7; inv H7.
-intros b H7 CONTRA.
-assert (H10: ~private_block (csem (active E s)) x b).
+intros b ofs H7 CONTRA.
+assert (H10: ~owned (csem (active E s)) x b ofs).
 assert (Hneq: j<>active E s) by auto.
  solve[apply (H2 j (active E s) d x Hneq H9 H1); auto].
 generalize H3 as H3'; intro.
-eapply private_newN in H3; eauto.
-specialize (VAL j d H9 b CONTRA).
+eapply owned_newN in H3; eauto.
+specialize (VAL j d H9 b ofs CONTRA).
 omega.
 inv Hcore_compatible.
 solve[erewrite corestep_others_backward; eauto].
 destruct (eq_nat_dec j (active E s)). subst.
 cut (proj_core E i s = Some c). intro H9.
 rewrite H5 in H8; inv H8.
-intros b H8 CONTRA.
-assert (H10: ~private_block (csem (active E s)) x b).
+intros b ofs H8 CONTRA.
+assert (H10: ~owned (csem (active E s)) x b ofs).
 assert (Hneq: i<>active E s) by auto.
  solve[apply (H2 i (active E s) c x Hneq H9 H1); auto].
 generalize H3 as H3'; intro.
-eapply private_newN in H3; eauto.
-specialize (VAL i c H9 b H8).
+eapply owned_newN in H3; eauto.
+specialize (VAL i c H9 b ofs H8).
 omega.
 inv Hcore_compatible.
 solve[erewrite corestep_others_backward; eauto].
@@ -457,7 +457,7 @@ Module ExtendedSimulations. Section ExtendedSimulations.
 
  Variable core_data: forall i: nat, Type.
  Variable match_state: forall i: nat, 
-   core_data i -> meminj -> cS i -> mem -> cT i -> mem -> Prop.
+   core_data i -> reserve_map -> meminj -> cS i -> mem -> cT i -> mem -> Prop.
  Variable core_ord: forall i: nat, core_data i -> core_data i -> Prop.
  Implicit Arguments match_state [].
  Implicit Arguments core_ord [].
@@ -470,7 +470,7 @@ Module ExtendedSimulations. Section ExtendedSimulations.
 
  Definition core_datas := forall i:nat, core_data i.
 
- Variable R: meminj -> xS -> mem -> xT -> mem -> Prop.
+ Variable R: reserve_map -> meminj -> xS -> mem -> xT -> mem -> Prop.
 
  Definition core_ords (max_cores: nat) cd1 cd2 := 
 (*exists i, (i < max_cores)%nat /\
@@ -502,119 +502,118 @@ Module ExtendedSimulations. Section ExtendedSimulations.
  solve[intros i; destruct (core_simulations i); auto].
  Qed.
 
- Definition match_states (cd: core_datas) (j: meminj) (s1: xS) m1 (s2: xT) m2 :=
-   private_valid esemS csemS E_S s1 m1 /\ private_disjoint esemS csemS E_S s1 /\ 
-   private_valid esemT csemT E_T s2 m2 /\ private_disjoint esemT csemT E_T s2 /\
-   R j s1 m1 s2 m2 /\ 
+ Definition match_states (cd: core_datas) (r: reserve_map) (j: meminj) (s1: xS) m1 (s2: xT) m2 :=
+   owned_valid esemS csemS E_S s1 m1 /\ owned_disjoint esemS csemS E_S s1 /\ 
+   owned_valid esemT csemT E_T s2 m2 /\ owned_disjoint esemT csemT E_T s2 /\
+   reserve_map_valid r m1 /\ reserve_map_valid r m2 /\
+   R r j s1 m1 s2 m2 /\ 
    ACTIVE E_S s1=ACTIVE E_T s2 /\
    forall i c1, PROJ_CORE E_S i s1 = Some c1 -> 
      exists c2, PROJ_CORE E_T i s2 = Some c2 /\ 
-       match_state i (cd i) j c1 m1 c2 m2.
+       match_state i (cd i) r j c1 m1 c2 m2.
 
  Variable max_cores: nat. (*TODO: fixme*)
 
  Inductive internal_compilability_invariant: Type := 
    InternalCompilabilityInvariant: forall 
-  (match_others: forall i cd j j' s1 cd' c1 m1 c1' m1' s2 c2 m2 c2' m2' d1 d2 n, 
+  (match_others: forall i cd r r' j j' s1 cd' c1 m1 c1' m1' s2 c2 m2 c2' m2' d1 d2 n, 
     PROJ_CORE E_S (ACTIVE E_S s1) s1 = Some c1 -> 
     PROJ_CORE E_T (ACTIVE E_S s1) s2 = Some c2 -> 
     PROJ_CORE E_S i s1 = Some d1 -> 
     PROJ_CORE E_T i s2 = Some d2 -> 
     ACTIVE E_S s1 <> i -> 
-    match_states cd j s1 m1 s2 m2 -> 
+    match_states cd r j s1 m1 s2 m2 -> 
     Mem.inject j m1 m2 -> 
     meminj_preserves_globals_ind (genv2blocks ge_S) j -> 
     inject_incr j j' -> 
     Events.inject_separated j j' m1 m2 -> 
+    reserve_map_incr r r' -> 
+    reserve_map_separated r r' m1 m2 -> 
     corestep (csemS (ACTIVE E_S s1)) (genv_mapS (ACTIVE E_S s1)) c1 m1 c1' m1' -> 
     corestepN (csemT (ACTIVE E_S s1)) (genv_mapT (ACTIVE E_S s1)) n c2 m2 c2' m2' -> 
-    match_state (ACTIVE E_S s1) cd' j' c1' m1' c2' m2' -> 
-    Events.mem_unchanged_on (fun b ofs => 
-      Events.loc_unmapped j b ofs /\ ~private_block (csemS (ACTIVE E_S s1)) c1 b) m1 m1' -> 
-    Events.mem_unchanged_on (fun b ofs => 
-      Events.loc_out_of_reach j m1 b ofs /\ ~private_block (csemT (ACTIVE E_S s1)) c2 b) m2 m2' -> 
-    match_state i (cd i) j' d1 m1' d2 m2')
+    match_state (ACTIVE E_S s1) cd' r' j' c1' m1' c2' m2' -> 
+    Events.mem_unchanged_on (guarantee_left (csemS (ACTIVE E_S s1)) r c1) m1 m1' -> 
+    Events.mem_unchanged_on (guarantee_right (csemS (ACTIVE E_S s1)) j r c1) m2 m2' -> 
+    match_state i (cd i) r' j' d1 m1' d2 m2')
 
-  (match_state_runnable: forall i cd j c1 m1 c2 m2,
-    match_state i cd j c1 m1 c2 m2 -> runnable (csemS i) c1=runnable (csemT i) c2)
+  (match_state_runnable: forall i cd r j c1 m1 c2 m2,
+    match_state i cd r j c1 m1 c2 m2 -> runnable (csemS i) c1=runnable (csemT i) c2)
 
-  (match_state_inj: forall i cd j c1 m1 c2 m2,
-    match_state i cd j c1 m1 c2 m2 -> Mem.inject j m1 m2)
+  (match_state_inj: forall i cd r j c1 m1 c2 m2,
+    match_state i cd r j c1 m1 c2 m2 -> Mem.inject j m1 m2)
 
-  (match_state_preserves_globals: forall i cd j c1 m1 c2 m2,
-    match_state i cd j c1 m1 c2 m2 -> 
+  (match_state_preserves_globals: forall i cd r j c1 m1 c2 m2,
+    match_state i cd r j c1 m1 c2 m2 -> 
     Events.meminj_preserves_globals (genv_mapS i) j)
 
-  (corestep_rel: forall cd j j' s1 c1 m1 c1' m1' s2 c2 m2 c2' m2' s1' s2' n cd', 
-    PROJ_CORE E_S (ACTIVE E_S s1) s1 = Some c1 -> 
-    PROJ_CORE E_T (ACTIVE E_S s1) s2 = Some c2 -> 
-    match_states cd j s1 m1 s2 m2 -> 
-    Mem.inject j m1 m2 -> 
-    meminj_preserves_globals_ind (genv2blocks ge_S) j -> 
-    inject_incr j j' -> 
-    Events.inject_separated j j' m1 m2 -> 
-    corestep (csemS (ACTIVE E_S s1)) (genv_mapS (ACTIVE E_S s1)) c1 m1 c1' m1' -> 
-    corestepN (csemT (ACTIVE E_S s1)) (genv_mapT (ACTIVE E_S s1)) n c2 m2 c2' m2' ->
-    corestep esemS ge_S s1 m1 s1' m1' -> 
-    corestepN esemT ge_T n s2 m2 s2' m2' -> 
-    match_state (ACTIVE E_S s1) cd' j' c1' m1' c2' m2' -> 
-    Events.mem_unchanged_on (fun b ofs => 
-      Events.loc_unmapped j b ofs /\ ~private_block (csemS (ACTIVE E_S s1)) c1 b) m1 m1' -> 
-    Events.mem_unchanged_on (fun b ofs => 
-      Events.loc_out_of_reach j m1 b ofs /\ ~private_block (csemT (ACTIVE E_S s1)) c2 b) m2 m2' -> 
-    R j' s1' m1' s2' m2')
-
- (after_external_rel: forall cd j j' s1 m1 s2 m2 s1' m1' s2' m2' ret1 ret2 ef sig args1,
-   match_states cd j s1 m1 s2 m2 -> 
+ (corestep_rel: forall cd r r' j j' s1 c1 m1 c1' m1' s2 c2 m2 c2' m2' s1' s2' n cd', 
+   PROJ_CORE E_S (ACTIVE E_S s1) s1 = Some c1 -> 
+   PROJ_CORE E_T (ACTIVE E_S s1) s2 = Some c2 -> 
+   match_states cd r j s1 m1 s2 m2 -> 
+   Mem.inject j m1 m2 -> 
+   meminj_preserves_globals_ind (genv2blocks ge_S) j -> 
    inject_incr j j' -> 
    Events.inject_separated j j' m1 m2 -> 
+   reserve_map_incr r r' -> 
+   reserve_map_separated r r' m1 m2 -> 
+   corestep (csemS (ACTIVE E_S s1)) (genv_mapS (ACTIVE E_S s1)) c1 m1 c1' m1' -> 
+   corestepN (csemT (ACTIVE E_S s1)) (genv_mapT (ACTIVE E_S s1)) n c2 m2 c2' m2' ->
+   corestep esemS ge_S s1 m1 s1' m1' -> 
+   corestepN esemT ge_T n s2 m2 s2' m2' -> 
+   match_state (ACTIVE E_S s1) cd' r' j' c1' m1' c2' m2' -> 
+   Events.mem_unchanged_on (guarantee_left (csemS (ACTIVE E_S s1)) r c1) m1 m1' -> 
+   Events.mem_unchanged_on (guarantee_right (csemS (ACTIVE E_S s1)) j r c1) m2 m2' -> 
+   R r' j' s1' m1' s2' m2')
+
+ (after_external_rel: forall cd r r' j j' s1 m1 s2 m2 s1' m1' s2' m2' ret1 ret2 ef sig args1,
+   match_states cd r j s1 m1 s2 m2 -> 
+   inject_incr j j' -> 
+   Events.inject_separated j j' m1 m2 -> 
+   reserve_map_incr r r' -> 
+   reserve_map_separated r r' m1 m2 -> 
    Mem.inject j' m1' m2' -> 
    mem_forward m1 m1'-> 
-   Events.mem_unchanged_on (fun b ofs => 
-     Events.loc_unmapped j b ofs /\ private_block esemS s1 b) m1 m1' -> 
    mem_forward m2 m2' -> 
-   Events.mem_unchanged_on (fun b ofs => 
-     Events.loc_out_of_reach j m1 b ofs /\ private_block esemT s2 b) m2 m2' -> 
+   Events.mem_unchanged_on (rely_left esemS r s1) m1 m1' -> 
+   Events.mem_unchanged_on (rely_right esemS j r s1) m2 m2' -> 
    at_external esemS s1 = Some (ef, sig, args1) -> 
    after_external esemS ret1 s1 = Some s1' -> 
    after_external esemT ret2 s2 = Some s2' -> 
    val_has_type_opt ret1 (ef_sig ef) -> 
    val_has_type_opt ret2 (ef_sig ef) -> 
    val_inject_opt j' ret1 ret2 -> 
-   R j' s1' m1' s2' m2')   
+   R r' j' s1' m1' s2' m2')   
  
- (extension_diagram: forall s1 m1 s1' m1' s2 c1 c2 m2 ef sig args1 args2 cd j,
+ (extension_diagram: forall s1 m1 s1' m1' s2 c1 c2 m2 ef sig args1 args2 cd r j,
    PROJ_CORE E_S (ACTIVE E_S s1) s1 = Some c1 -> 
    PROJ_CORE E_T (ACTIVE E_S s1) s2 = Some c2 -> 
    runnable (csemS (ACTIVE E_S s1)) c1=false -> 
    runnable (csemT (ACTIVE E_S s1)) c2=false -> 
    at_external (csemS (ACTIVE E_S s1)) c1 = Some (ef, sig, args1) -> 
    at_external (csemT (ACTIVE E_S s1)) c2 = Some (ef, sig, args2) -> 
-   match_states cd j s1 m1 s2 m2 -> 
+   match_states cd r j s1 m1 s2 m2 -> 
    Mem.inject j m1 m2 -> 
    Events.meminj_preserves_globals ge_S j -> 
    Forall2 (val_inject j) args1 args2 -> 
    Forall2 Val.has_type args2 (sig_args (ef_sig ef)) -> 
    corestep esemS ge_S s1 m1 s1' m1' -> 
-   exists s2', exists m2', exists cd', exists j',
+   exists s2', exists m2', exists cd', exists r', exists j',
      inject_incr j j' /\
      Events.inject_separated j j' m1 m2 /\
-     match_states cd' j' s1' m1' s2' m2' /\
-     Events.mem_unchanged_on (fun b ofs => 
-       Events.loc_unmapped j b ofs /\ ~private_block esemS s1 b) m1 m1' /\
-     Events.mem_unchanged_on (fun b ofs => 
-       Events.loc_out_of_reach j m1 b ofs /\ ~private_block esemT s2 b) m2 m2' /\
+     match_states cd' r' j' s1' m1' s2' m2' /\
+     Events.mem_unchanged_on (guarantee_left esemS r s1) m1 m1' /\
+     Events.mem_unchanged_on (guarantee_right esemS j r s1) m2 m2' /\
      ((corestep_plus esemT ge_T s2 m2 s2' m2') \/
       corestep_star esemT ge_T s2 m2 s2' m2' /\ core_ords max_cores cd' cd))
 
- (at_external_match: forall s1 m1 s2 c1 c2 m2 ef sig args1 args2 cd j,
+ (at_external_match: forall s1 m1 s2 c1 c2 m2 ef sig args1 args2 cd r j,
    ACTIVE E_S s1=ACTIVE E_T s2 -> 
    PROJ_CORE E_S (ACTIVE E_S s1) s1 = Some c1 -> 
    PROJ_CORE E_T (ACTIVE E_S s1) s2 = Some c2 -> 
    runnable (csemS (ACTIVE E_S s1)) c1=runnable (csemT (ACTIVE E_S s1)) c2 -> 
    at_external esemS s1 = Some (ef, sig, args1) -> 
    at_external (csemS (ACTIVE E_S s1)) c1 = Some (ef, sig, args1) -> 
-   match_state (ACTIVE E_S s1) cd j c1 m1 c2 m2 -> 
+   match_state (ACTIVE E_S s1) cd r j c1 m1 c2 m2 -> 
    Mem.inject j m1 m2 -> 
    Events.meminj_preserves_globals ge_S j -> 
    Forall2 (val_inject j) args1 args2 -> 
@@ -623,40 +622,43 @@ Module ExtendedSimulations. Section ExtendedSimulations.
    at_external esemT s2 = Some (ef, sig, args2))
 
  (after_external_diagram: 
-   forall i d1 s1 m1 d2 s2 m2 s1' m1' s2' m2' ef sig args1 retv1 retv2 cd j j',
-   match_state i cd j d1 m1 d2 m2 -> 
+   forall i d1 s1 m1 d2 s2 m2 s1' m1' s2' m2' ef sig args1 retv1 retv2 cd r r' j j',
+   match_state i cd r j d1 m1 d2 m2 -> 
    at_external esemS s1 = Some (ef, sig, args1) -> 
    Events.meminj_preserves_globals ge_S j -> 
    inject_incr j j' -> 
    Events.inject_separated j j' m1 m2 -> 
+   reserve_map_incr r r' -> 
+   reserve_map_separated r r' m1 m2 -> 
    Mem.inject j' m1' m2' -> 
    val_inject_opt j' retv1 retv2 -> 
    mem_forward m1 m1' -> 
-   Events.mem_unchanged_on (fun b ofs => 
-     Events.loc_unmapped j b ofs /\ private_block (csemS i) d1 b) m1 m1' -> 
    mem_forward m2 m2' -> 
-   Events.mem_unchanged_on (fun b ofs => 
-     Events.loc_out_of_reach j m1 b ofs /\ private_block (csemT i) d2 b) m2 m2' -> 
+   Events.mem_unchanged_on (rely_left (csemS i) r d1) m1 m1' ->  
+   Events.mem_unchanged_on (rely_right (csemS i) j r d1) m2 m2' -> 
    val_has_type_opt' retv2 (proj_sig_res (ef_sig ef)) -> 
    after_external esemS retv1 s1 = Some s1' -> 
    after_external esemT retv2 s2 = Some s2' -> 
    PROJ_CORE E_S i s1' = Some d1 -> 
    PROJ_CORE E_T i s2' = Some d2 -> 
    ACTIVE E_S s1 <> i -> 
-   match_state i cd j' d1 m1' d2 m2')
+   match_state i cd r' j' d1 m1' d2 m2')
 
-  (make_initial_core_diagram: forall v1 vals1 s1 m1 v2 vals2 m2 j sig,
-    In (v1, v2, sig) entry_points -> 
-    make_initial_core esemS ge_S v1 vals1 = Some s1 -> 
-    Mem.inject j m1 m2 -> 
-    Forall2 (val_inject j) vals1 vals2 -> 
-    Forall2 Val.has_type vals2 (sig_args sig) -> 
-    exists cd, exists s2, 
-      make_initial_core esemT ge_T v2 vals2 = Some s2 /\
-      match_states cd j s1 m1 s2 m2)
+
+ (make_initial_core_diagram: forall v1 vals1 s1 m1 v2 vals2 m2 r j sig,
+   In (v1, v2, sig) entry_points -> 
+   make_initial_core esemS ge_S v1 vals1 = Some s1 -> 
+   Mem.inject j m1 m2 -> 
+   reserve_map_valid r m1 -> 
+   reserve_map_valid r m2 -> 
+   Forall2 (val_inject j) vals1 vals2 -> 
+   Forall2 Val.has_type vals2 (sig_args sig) -> 
+   exists cd, exists s2, 
+                make_initial_core esemT ge_T v2 vals2 = Some s2 /\
+                match_states cd r j s1 m1 s2 m2)
  
- (safely_halted_step: forall cd j c1 m1 c2 m2 v1 rty,
-   match_states cd j c1 m1 c2 m2 -> 
+ (safely_halted_step: forall cd r j c1 m1 c2 m2 v1 rty,
+   match_states cd r j c1 m1 c2 m2 -> 
    safely_halted esemS c1 = Some v1 -> 
    Val.has_type v1 rty -> 
    exists v2, val_inject j v1 v2 /\
@@ -664,8 +666,8 @@ Module ExtendedSimulations. Section ExtendedSimulations.
      Val.has_type v2 rty /\ 
      Mem.inject j m1 m2)
 
- (safely_halted_diagram: forall cd j m1 m1' m2 rv1 s1 s2 s1' c1 c2,
-   match_states cd j s1 m1 s2 m2 -> 
+ (safely_halted_diagram: forall cd r j m1 m1' m2 rv1 s1 s2 s1' c1 c2,
+   match_states cd r j s1 m1 s2 m2 -> 
    PROJ_CORE E_S (ACTIVE E_S s1) s1 = Some c1 -> 
    PROJ_CORE E_T (ACTIVE E_S s1) s2 = Some c2 -> 
    safely_halted (csemS (ACTIVE E_S s1)) c1 = Some rv1 -> 
@@ -673,15 +675,15 @@ Module ExtendedSimulations. Section ExtendedSimulations.
    exists rv2, 
      safely_halted (csemT (ACTIVE E_S s1)) c2 = Some rv2 /\
      val_inject j rv1 rv2 /\ 
-   exists s2', exists m2', exists cd', exists j', 
+   exists s2', exists m2', exists cd', exists r', exists j', 
      inject_incr j j' /\
      Events.inject_separated j j' m1 m2 /\
+     reserve_map_incr r r' /\
+     reserve_map_separated r r' m1 m2 /\
      corestep esemT ge_T s2 m2 s2' m2' /\
-     match_states cd' j' s1' m1' s2' m2' /\
-     Events.mem_unchanged_on (fun b ofs => 
-       Events.loc_unmapped j b ofs /\ ~private_block (csemS (ACTIVE E_S s1)) c1 b) m1 m1' /\
-     Events.mem_unchanged_on (fun b ofs => 
-       Events.loc_out_of_reach j m1 b ofs /\ ~private_block (csemT (ACTIVE E_S s1)) c2 b) m2 m2'),
+     match_states cd' r' j' s1' m1' s2' m2' /\
+     Events.mem_unchanged_on (guarantee_left (csemS (ACTIVE E_S s1)) r c1) m1 m1' /\
+     Events.mem_unchanged_on (guarantee_right (csemS (ACTIVE E_S s1)) j r c1) m2 m2'),
   internal_compilability_invariant.
 
  Variables 
@@ -690,8 +692,8 @@ Module ExtendedSimulations. Section ExtendedSimulations.
   (genvs_domain_eqT: forall i: nat, genvs_domain_eq ge_T (genv_mapT i))
   (core_compatS: core_compatible ge_S genv_mapS E_S) 
   (core_compatT: core_compatible ge_T genv_mapT E_T)
-  (private_conservS: private_conserving esemS csemS E_S)
-  (private_conservT: private_conserving esemT csemT E_T)
+  (owned_conservS: owned_conserving esemS csemS E_S)
+  (owned_conservT: owned_conserving esemT csemT E_T)
   (active_okS: (forall x_s, ACTIVE E_S x_s < max_cores)%nat)
   (active_okT: (forall x_t, ACTIVE E_T x_t < max_cores)%nat).
 
@@ -700,12 +702,14 @@ Program Definition extended_simulation:
            entry_points core_datas match_states (core_ords max_cores) :=
   @Build_Forward_simulation_inject _ _ _ _ _ _ _ 
   esemS esemT ge_S ge_T entry_points core_datas match_states (core_ords max_cores) 
-  _ _ _ _ _ _.
+  _ _ _ _ _ _ _.
 Next Obligation. apply core_ords_wf. Qed.
+Next Obligation.
+split; auto.
 Next Obligation. 
 rename H0 into MATCH.
 generalize MATCH as MATCH'; intro.
-destruct MATCH as [VAL1 [DISJ1 [VAL2 [DISJ2 [RR [ACT MATCH_CORES]]]]]].
+destruct MATCH as [VAL1 [DISJ1 [VAL2 [DISJ2 [RVAL1 [RVAL2 [RR [ACT MATCH_CORES]]]]]]]].
 rename H into STEP.
 destruct (active_proj_core E_S st1) as [c1 PROJ1].
 destruct (active_proj_core E_T st2) as [c2 PROJ2].
@@ -724,7 +728,7 @@ intros RUN1.
 assert (RUN2: runnable (csemT (ACTIVE E_S st1)) c2=true).
  inv esig_compilable.
  rewrite match_state_runnable 
-  with (cd := cd (ACTIVE E_S st1)) (j := j) (m1 := m1) (c2 := c2) (m2 := m2) in RUN1.
+  with (cd := cd (ACTIVE E_S st1)) (r := r) (j := j) (m1 := m1) (c2 := c2) (m2 := m2) in RUN1.
  auto.
  specialize (MATCH_CORES (ACTIVE E_S st1) c1).
  spec MATCH_CORES; auto.
@@ -757,8 +761,9 @@ generalize (core_diagram (core_simulations (ACTIVE E_S st1))) as DIAG; intro.
 clear c2 PROJ2 RUN2.
 destruct (MATCH_CORES (ACTIVE E_S st1) c1 PROJ1) as [c2 [PROJ2 MATCH12]].
 unfold core_datas in cd.
-specialize (DIAG c1 m1 c1' m1' STEP1 (cd _) c2 j m2 MATCH12).
-destruct DIAG as [c2' [m2' [cd' [j' [INJ_INCR [INJ_SEP [MATCH12' [UNCH1 [UNCH2 STEP2]]]]]]]]].
+specialize (DIAG c1 m1 c1' m1' STEP1 (cd _) r c2 j m2 MATCH12).
+destruct DIAG as [c2' [m2' [cd' [r' [j' [INJ_INCR [INJ_SEP [RINCR [RSEP 
+ [MATCH12' [UNCH1 [UNCH2 STEP2]]]]]]]]]]]].
 destruct STEP2 as [STEP2|STEP2].
 
 (*corestep_plus case*)
@@ -772,35 +777,42 @@ spec CSTEPN; auto.
 destruct CSTEPN as [st2' [ESEM2 [ACT2' PROJ2']]].
 exists st2'; exists m2'.
 exists (core_datas_upd (ACTIVE E_S st1) cd' cd).
+exists r'.
 exists j'.
 split3; auto.
+split; auto.
+split; auto.
 split; auto.
  (*Subgoal: match_states*)
  hnf.
  split.
 
- (*private_valid*)
- eapply private_valid_inv with (n := S O); eauto.
+ (*owned_valid*)
+ eapply owned_valid_inv with (n := S O); eauto.
  solve[simpl; exists c1'; exists m1'; eauto].
  solve[simpl; eexists st1'; eexists m1'; eauto].
- (*private_disjoint*)
+ (*owned_disjoint*)
  split.
- eapply private_disjoint_inv with (n := S O) (m' := m1'); eauto.
+ eapply owned_disjoint_inv with (n := S O) (m' := m1'); eauto.
  solve[simpl; exists c1'; exists m1'; eauto].
  solve[simpl; eexists st1'; eexists m1'; eauto].
 
- (*private_valid*)
+ (*owned_valid*)
  split.
  forget (ACTIVE E_S st1) as k1.
  forget (ACTIVE E_T st2') as k2.
  subst.
- solve[eapply private_valid_inv; eauto].
- (*private_disjoint*)
+ solve[eapply owned_valid_inv; eauto].
+ (*owned_disjoint*)
  split.
  forget (ACTIVE E_S st1) as k1.
  forget (ACTIVE E_T st2') as k2.
  subst.
- solve[eapply private_disjoint_inv; eauto].
+ solve[eapply owned_disjoint_inv; eauto].
+
+ split.
+ destruct (core_simulations (ACTIVE E_S st1)).
+ eapply reserve_valid0.
 
  split.
  inv esig_compilable. 
@@ -877,21 +889,21 @@ split; auto.
    split.
    (*mem_unch_on unmapped*)
    apply mem_unchanged_on_sub with (Q := fun b ofs => 
-     loc_unmapped j b ofs /\ ~private_block (csemS (ACTIVE E_S st1)) c1 b); auto.
+     loc_unmapped j b ofs /\ ~owned (csemS (ACTIVE E_S st1)) c1 b); auto.
    intros b ofs [X Y]; split; auto.
    intros CONTRA; apply Y.
-   assert (private_block (csemS (ACTIVE E_S st1)) c1 b -> 
-           private_block esemS st1 b).
-    solve[apply private_conservS; auto].
+   assert (owned (csemS (ACTIVE E_S st1)) c1 b -> 
+           owned esemS st1 b).
+    solve[apply owned_conservS; auto].
    solve[auto].
    split.
    apply mem_unchanged_on_sub with (Q := fun b ofs => 
-     loc_out_of_reach j m1 b ofs /\ ~private_block (csemT (ACTIVE E_S st1)) c2 b); auto.
+     loc_out_of_reach j m1 b ofs /\ ~owned (csemT (ACTIVE E_S st1)) c2 b); auto.
    intros b ofs [X Y]; split; auto.
    intros CONTRA; apply Y.
-   assert (private_block (csemT (ACTIVE E_S st1)) c2 b -> 
-           private_block esemT st2 b).
-    solve[apply private_conservT; auto].
+   assert (owned (csemT (ACTIVE E_S st1)) c2 b -> 
+           owned esemT st2 b).
+    solve[apply owned_conservT; auto].
    solve[auto].
 
   solve[left; exists n; auto].
@@ -914,28 +926,28 @@ split; auto.
  hnf.
  split.
 
- (*private_valid*)
- eapply private_valid_inv with (n := S O); eauto.
+ (*owned_valid*)
+ eapply owned_valid_inv with (n := S O); eauto.
  solve[simpl; exists c1'; exists m1'; eauto].
  solve[simpl; eexists st1'; eexists m1'; eauto].
- (*private_disjoint*)
+ (*owned_disjoint*)
  split.
- eapply private_disjoint_inv with (n := S O) (m' := m1'); eauto.
+ eapply owned_disjoint_inv with (n := S O) (m' := m1'); eauto.
  solve[simpl; exists c1'; exists m1'; eauto].
  solve[simpl; eexists st1'; eexists m1'; eauto].
 
- (*private_valid*)
+ (*owned_valid*)
  split.
  forget (ACTIVE E_S st1) as k1.
  forget (ACTIVE E_T st2') as k2.
  subst.
- solve[eapply private_valid_inv; eauto].
- (*private_disjoint*)
+ solve[eapply owned_valid_inv; eauto].
+ (*owned_disjoint*)
  split.
  forget (ACTIVE E_S st1) as k1.
  forget (ACTIVE E_T st2') as k2.
  subst.
- solve[eapply private_disjoint_inv; eauto].
+ solve[eapply owned_disjoint_inv; eauto].
 
  split.
  inv esig_compilable. 
@@ -1012,21 +1024,21 @@ split; auto.
   split. 
   (*mem_unch_on unmapped*)
   apply mem_unchanged_on_sub with (Q := fun b ofs => 
-    loc_unmapped j b ofs /\ ~private_block (csemS (ACTIVE E_S st1)) c1 b); auto.
+    loc_unmapped j b ofs /\ ~owned (csemS (ACTIVE E_S st1)) c1 b); auto.
   intros b ofs [X Y]; split; auto.
   intros CONTRA; apply Y.
-  assert (private_block (csemS (ACTIVE E_S st1)) c1 b -> 
-          private_block esemS st1 b).
-   solve[apply private_conservS; auto].
+  assert (owned (csemS (ACTIVE E_S st1)) c1 b -> 
+          owned esemS st1 b).
+   solve[apply owned_conservS; auto].
   solve[auto].
   split.
   apply mem_unchanged_on_sub with (Q := fun b ofs => 
-    loc_out_of_reach j m1 b ofs /\ ~private_block (csemT (ACTIVE E_S st1)) c2 b); auto.
+    loc_out_of_reach j m1 b ofs /\ ~owned (csemT (ACTIVE E_S st1)) c2 b); auto.
   intros b ofs [X Y]; split; auto.
   intros CONTRA; apply Y.
-  assert (private_block (csemT (ACTIVE E_S st1)) c2 b -> 
-          private_block esemT st2 b).
-   solve[apply private_conservT; auto].
+  assert (owned (csemT (ACTIVE E_S st1)) c2 b -> 
+          owned esemT st2 b).
+   solve[apply owned_conservT; auto].
   solve[auto].
 
   right. split. exists n. auto. 
@@ -1058,19 +1070,19 @@ split3; auto.
 
 apply mem_unchanged_on_sub with (Q := fun b ofs => 
   loc_unmapped j b ofs /\
-  ~private_block (csemS (ACTIVE E_S st1)) c1 b); auto.
+  ~owned (csemS (ACTIVE E_S st1)) c1 b); auto.
 intros b ofs [? ?]; split; auto.
 intros CONTRA.
 apply H0.
-solve[eapply private_conservS in CONTRA; eauto].
+solve[eapply owned_conservS in CONTRA; eauto].
 
 apply mem_unchanged_on_sub with (Q := fun b ofs => 
   loc_out_of_reach j m1 b ofs /\
-  ~private_block (csemT (ACTIVE E_S st1)) c2 b); auto.
+  ~owned (csemT (ACTIVE E_S st1)) c2 b); auto.
 intros b ofs [? ?]; split; auto.
 intros CONTRA.
 apply H0.
-solve[eapply private_conservT in CONTRA; eauto].
+solve[eapply owned_conservT in CONTRA; eauto].
 
 solve[left; exists 0%nat; eexists; eexists; split; simpl; eauto].
 
@@ -1142,15 +1154,15 @@ rewrite <-genvs_domain_eq_preserves with (ge1 := ge_S); auto.
 rewrite meminj_preserves_genv2blocks; auto.
 
 apply mem_unchanged_on_sub with (Q := fun b ofs => 
-  loc_unmapped j b ofs /\ private_block esemS st1 b); auto.
+  loc_unmapped j b ofs /\ owned esemS st1 b); auto.
 intros b ofs [? ?].
 split; auto.
-solve[eapply private_conservS; eauto].
+solve[eapply owned_conservS; eauto].
 apply mem_unchanged_on_sub with (Q := fun b ofs => 
-  loc_out_of_reach j m1 b ofs /\ private_block esemT st2 b); auto.
+  loc_out_of_reach j m1 b ofs /\ owned esemT st2 b); auto.
 intros b ofs [? ?].
 split; auto.
-solve[eapply private_conservT; eauto].
+solve[eapply owned_conservT; eauto].
 
 exists (core_datas_upd (ACTIVE E_S st1) cd' cd).
 assert (exists st1', after_external esemS ret1 st1 = Some st1' /\
@@ -1178,13 +1190,13 @@ assert (ACTIVE E_T st2=ACTIVE E_T st2') as <-.
  solve[eapply after_ext_pres; eauto].
 split; auto.
 
-(*private_valid*)
-solve[eapply private_valid_after_ext; eauto].
+(*owned_valid*)
+solve[eapply owned_valid_after_ext; eauto].
 split.
-(*private_disjoint*)
-solve[eapply private_disjoint_after_ext; eauto].
+(*owned_disjoint*)
+solve[eapply owned_disjoint_after_ext; eauto].
 split.
-(*private_valid*)
+(*owned_valid*)
 remember (ACTIVE E_S st1) as x.
 remember (ACTIVE E_S st1') as x'.
 remember (ACTIVE E_T st2') as y'.
@@ -1196,8 +1208,8 @@ assert (AT_EXT2: exists vals2,
  destruct AT_EXT1 as [_ [_ [vals2 [_ [_ AT_EXT2]]]]].
  exists vals2; eauto.
  destruct AT_EXT2 as [vals2 AT_EXT2].
- solve[eapply private_valid_after_ext; eauto].
-(*private_disjoint*)
+ solve[eapply owned_valid_after_ext; eauto].
+(*owned_disjoint*)
 remember (ACTIVE E_S st1) as x.
 remember (ACTIVE E_S st1') as x'.
 remember (ACTIVE E_T st2') as y'.
@@ -1210,7 +1222,7 @@ assert (AT_EXT2: exists vals2,
  exists vals2; eauto.
 destruct AT_EXT2 as [vals2 AT_EXT2].
 split.
-solve[eapply private_disjoint_after_ext; eauto].
+solve[eapply owned_disjoint_after_ext; eauto].
 
 split.
 inv esig_compilable.
@@ -1248,17 +1260,17 @@ eapply after_external_diagram; eauto.
 inv core_compatS.
 erewrite <-after_ext_others in _PROJ1'; eauto.
 apply mem_unchanged_on_sub with (Q := fun b ofs => 
-  loc_unmapped j b ofs /\ private_block esemS st1 b); auto.
+  loc_unmapped j b ofs /\ owned esemS st1 b); auto.
 intros b ofs [? ?].
 split; auto.
-apply private_conservS in _PROJ1'.
+apply owned_conservS in _PROJ1'.
 solve[eapply _PROJ1'; eauto].
 apply mem_unchanged_on_sub with (Q := fun b ofs => 
-  loc_out_of_reach j m1 b ofs /\ private_block esemT st2 b); auto.
+  loc_out_of_reach j m1 b ofs /\ owned esemT st2 b); auto.
 intros b ofs [? ?].
 split; auto.
 inv core_compatT.
-apply private_conservT in _PROJ2.
+apply owned_conservT in _PROJ2.
 solve[eapply _PROJ2; eauto].
 auto.
 inv core_compatT.
@@ -1297,15 +1309,15 @@ apply RELY; auto.
 erewrite <-genvs_domain_eq_preserves; eauto.
 solve[eapply match_state_inj; eauto].
 apply mem_unchanged_on_sub with (Q := fun b ofs => 
-  loc_unmapped j b ofs /\ ~private_block (csemS k) c1 b); auto.
+  loc_unmapped j b ofs /\ ~owned (csemS k) c1 b); auto.
 intros b ofs [X Y].
 split; auto.
-solve[unfold private_disjoint in DISJ1; eapply DISJ1; eauto].
+solve[unfold owned_disjoint in DISJ1; eapply DISJ1; eauto].
 apply mem_unchanged_on_sub with (Q := fun b ofs => 
-  loc_out_of_reach j m1 b ofs /\ ~private_block (csemT k) c2 b); auto.
+  loc_out_of_reach j m1 b ofs /\ ~owned (csemT k) c2 b); auto.
 intros b ofs [X Y].
 split; auto.
-solve[unfold private_disjoint in DISJ2; eapply DISJ2; eauto].
+solve[unfold owned_disjoint in DISJ2; eapply DISJ2; eauto].
 
 (*2*)
 intros; destruct (core_simulations_RGinject i) as [? _ _ _ _].
